src/FiniteSetADTs/WordInterface.v
@@ -1,5 +1,6 @@
 (** Before we integrated bedrock, we used a dummy implementation of
     this module using [nat]; see NatWord.v. *)
+Require Import Coq.Classes.Morphisms.
 
 Set Implicit Arguments.
 
@@ -7,6 +8,7 @@ Module Type BedrockWordT.
   Axiom W : Type.
   Axiom wzero : W.
   Axiom wplus : W -> W -> W.
+  Axiom wminus : W -> W -> W.
   Axiom weq : W -> W -> bool.
   Axiom wlt : W -> W -> bool.
   Axiom weq_iff : forall x y, x = y <-> weq x y = true.
@@ -14,4 +16,5 @@ Module Type BedrockWordT.
   Axiom wlt_trans : forall x y z, wlt x y = true -> wlt y z = true -> wlt x z = true.
   Axiom wle_antisym : forall x y, wlt x y = false -> wlt y x = false -> x = y.
   Axiom wle_asym : forall x y, wlt x y = true -> wlt y x = false.
+  Axiom from_nat : nat -> W.
 End BedrockWordT.
